basic fixes

w64x4/test/Fp_w64x4.c
@@ -21,14 +21,14 @@ extern void __expm(uint64_t* r, uint64_t* p, uint64_t* a, uint64_t* b);
 /*    } */
 /*  }; */
 
-uint64_t tmul[][4][64] =
- {
-  {  { 0ull , 0ull , 0ull , 0ull, 0ull , 0ull , 0ull , 0ull, 0ull , 0ull , 0ull , 0ull, 0ull , 0ull , 0ull , 0ull, 0ull , 0ull , 0ull , 0ull, 0ull , 0ull , 0ull , 0ull, 0ull , 0ull , 0ull , 0ull, 0ull , 0ull , 0ull , 0ull, 0ull , 0ull , 0ull , 0ull, 0ull , 0ull , 0ull , 0ull, 0ull , 0ull , 0ull , 0ull, 0ull , 0ull , 0ull , 0ull, 0ull , 0ull , 0ull , 0ull, 0ull , 0ull , 0ull , 0ull, 0ull , 0ull , 0ull , 0ull, 0ull , 0ull , 0ull , 0ull }
-     , { 0ull , 0ull , 0ull , 0ull, 0ull , 0ull , 0ull , 0ull, 0ull , 0ull , 0ull , 0ull, 0ull , 0ull , 0ull , 0ull, 0ull , 0ull , 0ull , 0ull, 0ull , 0ull , 0ull , 0ull, 0ull , 0ull , 0ull , 0ull, 0ull , 0ull , 0ull , 0ull, 0ull , 0ull , 0ull , 0ull, 0ull , 0ull , 0ull , 0ull, 0ull , 0ull , 0ull , 0ull, 0ull , 0ull , 0ull , 0ull, 0ull , 0ull , 0ull , 0ull, 0ull , 0ull , 0ull , 0ull, 0ull , 0ull , 0ull , 0ull, 0ull , 0ull , 0ull , 0ull }
-     , { 0ull , 0ull , 0ull , 0ull, 0ull , 0ull , 0ull , 0ull, 0ull , 0ull , 0ull , 0ull, 0ull , 0ull , 0ull , 0ull, 0ull , 0ull , 0ull , 0ull, 0ull , 0ull , 0ull , 0ull, 0ull , 0ull , 0ull , 0ull, 0ull , 0ull , 0ull , 0ull, 0ull , 0ull , 0ull , 0ull, 0ull , 0ull , 0ull , 0ull, 0ull , 0ull , 0ull , 0ull, 0ull , 0ull , 0ull , 0ull, 0ull , 0ull , 0ull , 0ull, 0ull , 0ull , 0ull , 0ull, 0ull , 0ull , 0ull , 0ull, 0ull , 0ull , 0ull , 0ull }
-     , { 0ull , 0ull , 0ull , 0ull, 0ull , 0ull , 0ull , 0ull, 0ull , 0ull , 0ull , 0ull, 0ull , 0ull , 0ull , 0ull, 0ull , 0ull , 0ull , 0ull, 0ull , 0ull , 0ull , 0ull, 0ull , 0ull , 0ull , 0ull, 0ull , 0ull , 0ull , 0ull, 0ull , 0ull , 0ull , 0ull, 0ull , 0ull , 0ull , 0ull, 0ull , 0ull , 0ull , 0ull, 0ull , 0ull , 0ull , 0ull, 0ull , 0ull , 0ull , 0ull, 0ull , 0ull , 0ull , 0ull, 0ull , 0ull , 0ull , 0ull, 0ull , 0ull , 0ull , 0ull }
-   }
- };
+/* uint64_t tmul[][4][64] = */
+/*  { */
+/*   {  { 0ull , 0ull , 0ull , 0ull, 0ull , 0ull , 0ull , 0ull, 0ull , 0ull , 0ull , 0ull, 0ull , 0ull , 0ull , 0ull, 0ull , 0ull , 0ull , 0ull, 0ull , 0ull , 0ull , 0ull, 0ull , 0ull , 0ull , 0ull, 0ull , 0ull , 0ull , 0ull, 0ull , 0ull , 0ull , 0ull, 0ull , 0ull , 0ull , 0ull, 0ull , 0ull , 0ull , 0ull, 0ull , 0ull , 0ull , 0ull, 0ull , 0ull , 0ull , 0ull, 0ull , 0ull , 0ull , 0ull, 0ull , 0ull , 0ull , 0ull, 0ull , 0ull , 0ull , 0ull } */
+/*      , { 0ull , 0ull , 0ull , 0ull, 0ull , 0ull , 0ull , 0ull, 0ull , 0ull , 0ull , 0ull, 0ull , 0ull , 0ull , 0ull, 0ull , 0ull , 0ull , 0ull, 0ull , 0ull , 0ull , 0ull, 0ull , 0ull , 0ull , 0ull, 0ull , 0ull , 0ull , 0ull, 0ull , 0ull , 0ull , 0ull, 0ull , 0ull , 0ull , 0ull, 0ull , 0ull , 0ull , 0ull, 0ull , 0ull , 0ull , 0ull, 0ull , 0ull , 0ull , 0ull, 0ull , 0ull , 0ull , 0ull, 0ull , 0ull , 0ull , 0ull, 0ull , 0ull , 0ull , 0ull } */
+/*      , { 0ull , 0ull , 0ull , 0ull, 0ull , 0ull , 0ull , 0ull, 0ull , 0ull , 0ull , 0ull, 0ull , 0ull , 0ull , 0ull, 0ull , 0ull , 0ull , 0ull, 0ull , 0ull , 0ull , 0ull, 0ull , 0ull , 0ull , 0ull, 0ull , 0ull , 0ull , 0ull, 0ull , 0ull , 0ull , 0ull, 0ull , 0ull , 0ull , 0ull, 0ull , 0ull , 0ull , 0ull, 0ull , 0ull , 0ull , 0ull, 0ull , 0ull , 0ull , 0ull, 0ull , 0ull , 0ull , 0ull, 0ull , 0ull , 0ull , 0ull, 0ull , 0ull , 0ull , 0ull } */
+/*      , { 0ull , 0ull , 0ull , 0ull, 0ull , 0ull , 0ull , 0ull, 0ull , 0ull , 0ull , 0ull, 0ull , 0ull , 0ull , 0ull, 0ull , 0ull , 0ull , 0ull, 0ull , 0ull , 0ull , 0ull, 0ull , 0ull , 0ull , 0ull, 0ull , 0ull , 0ull , 0ull, 0ull , 0ull , 0ull , 0ull, 0ull , 0ull , 0ull , 0ull, 0ull , 0ull , 0ull , 0ull, 0ull , 0ull , 0ull , 0ull, 0ull , 0ull , 0ull , 0ull, 0ull , 0ull , 0ull , 0ull, 0ull , 0ull , 0ull , 0ull, 0ull , 0ull , 0ull , 0ull } */
+/*    } */
+/*  }; */
 
 
 uint64_t texp[][4][64] =
@@ -101,41 +101,17 @@ int main(void) {
   uint64_t result[64]; 
   int i, b,a;
 
-  /* printf("Testing ADDM: "); */
-  /* b = 1; */
-  /* for (i=0; i<sizeof(tadd)/sizeof(tadd[0]); i++) { */
-  /*   __addm(result, tadd[i][0], tadd[i][1], tadd[i][2]); */
-  /*  a = memcmp(result, tadd[i][3], sizeof(tadd[i][3])); */
-  /*  b =   b && !a; */
-  /* } */
-  /* if (b) printf("OK\n"); else printf("FAIL!\n"); */
-
-
-    /* __mulm(result, tmul[3][0], tmul[3][1],tmul[3][2]); */
-    /* print_result(result); */
-  
-  /* printf("Testing MULM: "); */
-  /* b = 1; */
-  /* for (i=0; i<100000; i++) { */
-  /*   __mulm(result, tmul[0][0], tmul[i][1],tmul[0][2]); */
-  /*  a = memcmp(result, tmul[0][3], sizeof(tmul[0][3])); */
-  /*  b =   b && !a; */
-  /* } */
-  /* if (b) printf("OK\n"); else printf("FAIL!\n"); */
-
-
-  printf("Testing EXPM: ");
+  //  printf("Testing EXPM: ");
   b = 1;
-  //  for (i=0; i<sizeof(texp)/sizeof(texp[0]); i++) {
   for (i=0; i<1; i++) {
     __expm(result, texp[0][0], texp[0][1],texp[0][2]);
-   a = memcmp(result, texp[0][3], sizeof(texp[0][3]));
-   b =   b && !a;
+    //   a = memcmp(result, texp[0][3], sizeof(texp[0][3]));
+   //   b =   b && !a;
   }
-  if (b) printf("OK\n"); else printf("FAIL!\n");
+  //if (b) printf("OK\n"); else printf("FAIL!\n");
 
   
-  print_result(result);  
+  //  print_result(result);  
   
   return 0;
 }
