w64x4/proof/Fp_w64x4_extract_ct.ec
@@ -1,16 +1,15 @@
 require import AllCore IntDiv CoreMap List Distr.
 from Jasmin require import JModel.
 
-require import Array32.
-require import WArray256.
+require import Array4 Array8 Array16.
+require import WArray32 WArray64 WArray128.
 
 
 
 module M = {
   var leakages : leakages_t
   
-  proc bn_subc (a:W64.t Array32.t, b:W64.t Array32.t) : bool *
-                                                        W64.t Array32.t = {
+  proc dbn_subc (a:W64.t Array8.t, b:W64.t Array8.t) : bool * W64.t Array8.t = {
     var aux_0: bool;
     var aux_1: int;
     var aux: W64.t;
@@ -34,9 +33,9 @@ module M = {
     aux <- x1;
     leakages <- LeakAddr([0]) :: leakages;
     a.[0] <- aux;
-    leakages <- LeakFor(1,32) :: LeakAddr([]) :: leakages;
+    leakages <- LeakFor(1,8) :: LeakAddr([]) :: leakages;
     i <- 1;
-    while (i < 32) {
+    while (i < 8) {
       leakages <- LeakAddr([i]) :: leakages;
       aux <- a.[i];
       x1 <- aux;
@@ -56,17 +55,17 @@ module M = {
     return (cf, a);
   }
   
-  proc bn_copy (a:W64.t Array32.t) : W64.t Array32.t = {
+  proc bn_copy (a:W64.t Array4.t) : W64.t Array4.t = {
     var aux: int;
     var aux_0: W64.t;
     
-    var r:W64.t Array32.t;
+    var r:W64.t Array4.t;
     var i:int;
     var t:W64.t;
     r <- witness;
-    leakages <- LeakFor(0,32) :: LeakAddr([]) :: leakages;
+    leakages <- LeakFor(0,4) :: LeakAddr([]) :: leakages;
     i <- 0;
-    while (i < 32) {
+    while (i < 4) {
       leakages <- LeakAddr([i]) :: leakages;
       aux_0 <- a.[i];
       t <- aux_0;
@@ -79,15 +78,38 @@ module M = {
     return (r);
   }
   
-  proc bn_set0 (a:W64.t Array32.t) : W64.t Array32.t = {
+  proc dbn_copy (a:W64.t Array8.t) : W64.t Array8.t = {
+    var aux: int;
+    var aux_0: W64.t;
+    
+    var r:W64.t Array8.t;
+    var i:int;
+    var t:W64.t;
+    r <- witness;
+    leakages <- LeakFor(0,8) :: LeakAddr([]) :: leakages;
+    i <- 0;
+    while (i < 8) {
+      leakages <- LeakAddr([i]) :: leakages;
+      aux_0 <- a.[i];
+      t <- aux_0;
+      leakages <- LeakAddr([]) :: leakages;
+      aux_0 <- t;
+      leakages <- LeakAddr([i]) :: leakages;
+      r.[i] <- aux_0;
+      i <- i + 1;
+    }
+    return (r);
+  }
+  
+  proc bn_set0 (a:W64.t Array4.t) : W64.t Array4.t = {
     var aux: int;
     var aux_0: W64.t;
     
     var i:int;
     
-    leakages <- LeakFor(0,32) :: LeakAddr([]) :: leakages;
+    leakages <- LeakFor(0,4) :: LeakAddr([]) :: leakages;
     i <- 0;
-    while (i < 32) {
+    while (i < 4) {
       leakages <- LeakAddr([]) :: leakages;
       aux_0 <- (W64.of_int 0);
       leakages <- LeakAddr([i]) :: leakages;
@@ -97,55 +119,545 @@ module M = {
     return (a);
   }
   
-  proc bn_addc (a:W64.t Array32.t, b:W64.t Array32.t) : bool *
-                                                        W64.t Array32.t = {
-    var aux_0: bool;
-    var aux_1: int;
-    var aux: W64.t;
+  proc bn2_set0 (a:W64.t Array8.t) : W64.t Array8.t = {
+    var aux: int;
+    var aux_0: W64.t;
     
+    var i:int;
+    
+    leakages <- LeakFor(0,(2 * 4)) :: LeakAddr([]) :: leakages;
+    aux <- (2 * 4);
+    i <- 0;
+    while (i < aux) {
+      leakages <- LeakAddr([]) :: leakages;
+      aux_0 <- (W64.of_int 0);
+      leakages <- LeakAddr([i]) :: leakages;
+      a.[i] <- aux_0;
+      i <- i + 1;
+    }
+    return (a);
+  }
+  
+  proc mul1 (a:W64.t, b:W64.t Array4.t) : W64.t * bool * bool *
+                                          W64.t Array8.t = {
+    var aux_3: bool;
+    var aux_2: bool;
+    var aux_1: bool;
+    var aux_0: bool;
+    var aux: bool;
+    var aux_6: int;
+    var aux_5: W64.t;
+    var aux_4: W64.t;
+    
+    var _zero:W64.t;
+    var of_0:bool;
     var cf:bool;
+    var r:W64.t Array8.t;
     var x1:W64.t;
     var x2:W64.t;
     var i:int;
-    
-    leakages <- LeakAddr([0]) :: leakages;
-    aux <- a.[0];
-    x1 <- aux;
-    leakages <- LeakAddr([0]) :: leakages;
-    aux <- b.[0];
-    x2 <- aux;
+    var lo:W64.t;
+    var  _0:bool;
+    var  _1:bool;
+    var  _2:bool;
+    r <- witness;
     leakages <- LeakAddr([]) :: leakages;
-    (aux_0, aux) <- adc_64 x1 x2 false;
-    cf <- aux_0;
-    x1 <- aux;
+    (aux_3, aux_2, aux_1, aux_0, aux, aux_5) <- set0_64 ;
+    of_0 <- aux_3;
+    cf <- aux_2;
+     _0 <- aux_1;
+     _1 <- aux_0;
+     _2 <- aux;
+    _zero <- aux_5;
     leakages <- LeakAddr([]) :: leakages;
-    aux <- x1;
+    aux_5 <- a;
+    x1 <- aux_5;
     leakages <- LeakAddr([0]) :: leakages;
-    a.[0] <- aux;
-    leakages <- LeakFor(1,32) :: LeakAddr([]) :: leakages;
+    aux_5 <- b.[0];
+    x2 <- aux_5;
+    leakages <- LeakAddr([]) :: leakages;
+    (aux_5, aux_4) <- MULX_64 x1 x2;
+    x1 <- aux_5;
+    x2 <- aux_4;
+    leakages <- LeakAddr([]) :: leakages;
+    aux_5 <- x1;
+    leakages <- LeakAddr([1]) :: leakages;
+    r.[1] <- aux_5;
+    leakages <- LeakAddr([]) :: leakages;
+    aux_5 <- x2;
+    leakages <- LeakAddr([0]) :: leakages;
+    r.[0] <- aux_5;
+    leakages <- LeakFor(1,4) :: LeakAddr([]) :: leakages;
     i <- 1;
-    while (i < 32) {
-      leakages <- LeakAddr([i]) :: leakages;
-      aux <- a.[i];
-      x1 <- aux;
-      leakages <- LeakAddr([i]) :: leakages;
-      aux <- b.[i];
-      x2 <- aux;
+    while (i < 4) {
       leakages <- LeakAddr([]) :: leakages;
-      (aux_0, aux) <- adc_64 x1 x2 cf;
-      cf <- aux_0;
-      x1 <- aux;
-      leakages <- LeakAddr([]) :: leakages;
-      aux <- x1;
+      aux_5 <- a;
+      x1 <- aux_5;
       leakages <- LeakAddr([i]) :: leakages;
-      a.[i] <- aux;
+      aux_5 <- b.[i];
+      x2 <- aux_5;
+      leakages <- LeakAddr([]) :: leakages;
+      (aux_5, aux_4) <- MULX_64 x1 x2;
+      x1 <- aux_5;
+      x2 <- aux_4;
+      leakages <- LeakAddr([]) :: leakages;
+      aux_5 <- x1;
+      leakages <- LeakAddr([(i + 1)]) :: leakages;
+      r.[(i + 1)] <- aux_5;
+      leakages <- LeakAddr([]) :: leakages;
+      aux_5 <- x2;
+      lo <- aux_5;
+      leakages <- LeakAddr([i]) :: leakages;
+      aux_5 <- r.[i];
+      x1 <- aux_5;
+      leakages <- LeakAddr([]) :: leakages;
+      aux_5 <- lo;
+      x2 <- aux_5;
+      leakages <- LeakAddr([]) :: leakages;
+      (aux_3, aux_5) <- ADCX_64 x1 x2 cf;
+      cf <- aux_3;
+      x1 <- aux_5;
+      leakages <- LeakAddr([]) :: leakages;
+      aux_5 <- x1;
+      leakages <- LeakAddr([i]) :: leakages;
+      r.[i] <- aux_5;
       i <- i + 1;
     }
-    return (cf, a);
+    leakages <- LeakAddr([4]) :: leakages;
+    aux_5 <- r.[4];
+    x1 <- aux_5;
+    leakages <- LeakAddr([]) :: leakages;
+    (aux_3, aux_5) <- ADCX_64 x1 _zero cf;
+    cf <- aux_3;
+    x1 <- aux_5;
+    leakages <- LeakAddr([]) :: leakages;
+    aux_5 <- x1;
+    leakages <- LeakAddr([4]) :: leakages;
+    r.[4] <- aux_5;
+    return (_zero, of_0, cf, r);
   }
   
-  proc swapr (x:W64.t Array32.t, y:W64.t Array32.t, swap_0:W64.t) : W64.t Array32.t *
-                                                                    W64.t Array32.t = {
+  proc mul1acc (k:W64.t, a:W64.t, b:W64.t Array4.t, r:W64.t Array8.t,
+                _zero:W64.t, of_0:bool, cf:bool) : W64.t * bool * bool *
+                                                   W64.t Array8.t = {
+    var aux_2: bool;
+    var aux: int;
+    var aux_1: W64.t;
+    var aux_0: W64.t;
+    
+    var kk:int;
+    var x1:W64.t;
+    var i:int;
+    var x2:W64.t;
+    var hi:W64.t;
+    var lo:W64.t;
+    
+    leakages <- LeakAddr([]) :: leakages;
+    aux <- (W64.to_uint k);
+    kk <- aux;
+    leakages <- LeakFor(0,(4 - 1)) :: LeakAddr([]) :: leakages;
+    aux <- (4 - 1);
+    i <- 0;
+    while (i < aux) {
+      leakages <- LeakAddr([]) :: leakages;
+      aux_1 <- a;
+      x1 <- aux_1;
+      leakages <- LeakAddr([i]) :: leakages;
+      aux_1 <- b.[i];
+      x2 <- aux_1;
+      leakages <- LeakAddr([]) :: leakages;
+      (aux_1, aux_0) <- MULX_64 x1 x2;
+      x1 <- aux_1;
+      x2 <- aux_0;
+      leakages <- LeakAddr([]) :: leakages;
+      aux_1 <- x1;
+      hi <- aux_1;
+      leakages <- LeakAddr([]) :: leakages;
+      aux_1 <- x2;
+      lo <- aux_1;
+      leakages <- LeakAddr([(kk + i)]) :: leakages;
+      aux_1 <- r.[(kk + i)];
+      x1 <- aux_1;
+      leakages <- LeakAddr([]) :: leakages;
+      (aux_2, aux_1) <- ADOX_64 x1 lo of_0;
+      of_0 <- aux_2;
+      x1 <- aux_1;
+      leakages <- LeakAddr([]) :: leakages;
+      aux_1 <- x1;
+      leakages <- LeakAddr([(kk + i)]) :: leakages;
+      r.[(kk + i)] <- aux_1;
+      leakages <- LeakAddr([((kk + i) + 1)]) :: leakages;
+      aux_1 <- r.[((kk + i) + 1)];
+      x1 <- aux_1;
+      leakages <- LeakAddr([]) :: leakages;
+      (aux_2, aux_1) <- ADCX_64 x1 hi cf;
+      cf <- aux_2;
+      x1 <- aux_1;
+      leakages <- LeakAddr([]) :: leakages;
+      aux_1 <- x1;
+      leakages <- LeakAddr([((kk + i) + 1)]) :: leakages;
+      r.[((kk + i) + 1)] <- aux_1;
+      i <- i + 1;
+    }
+    leakages <- LeakAddr([]) :: leakages;
+    aux_1 <- a;
+    x1 <- aux_1;
+    leakages <- LeakAddr([(4 - 1)]) :: leakages;
+    aux_1 <- b.[(4 - 1)];
+    x2 <- aux_1;
+    leakages <- LeakAddr([]) :: leakages;
+    (aux_1, aux_0) <- MULX_64 x1 x2;
+    x1 <- aux_1;
+    x2 <- aux_0;
+    leakages <- LeakAddr([]) :: leakages;
+    aux_1 <- x1;
+    leakages <- LeakAddr([(4 + kk)]) :: leakages;
+    r.[(4 + kk)] <- aux_1;
+    leakages <- LeakAddr([]) :: leakages;
+    aux_1 <- x2;
+    lo <- aux_1;
+    leakages <- LeakAddr([((4 + kk) - 1)]) :: leakages;
+    aux_1 <- r.[((4 + kk) - 1)];
+    x1 <- aux_1;
+    leakages <- LeakAddr([]) :: leakages;
+    (aux_2, aux_1) <- ADOX_64 x1 lo of_0;
+    of_0 <- aux_2;
+    x1 <- aux_1;
+    leakages <- LeakAddr([]) :: leakages;
+    aux_1 <- x1;
+    leakages <- LeakAddr([((4 + kk) - 1)]) :: leakages;
+    r.[((4 + kk) - 1)] <- aux_1;
+    leakages <- LeakAddr([(4 + kk)]) :: leakages;
+    aux_1 <- r.[(4 + kk)];
+    x1 <- aux_1;
+    leakages <- LeakAddr([]) :: leakages;
+    (aux_2, aux_1) <- ADCX_64 x1 _zero cf;
+    cf <- aux_2;
+    x1 <- aux_1;
+    leakages <- LeakAddr([]) :: leakages;
+    aux_1 <- x1;
+    leakages <- LeakAddr([(4 + kk)]) :: leakages;
+    r.[(4 + kk)] <- aux_1;
+    leakages <- LeakAddr([(4 + kk)]) :: leakages;
+    aux_1 <- r.[(4 + kk)];
+    x1 <- aux_1;
+    leakages <- LeakAddr([]) :: leakages;
+    (aux_2, aux_1) <- ADOX_64 x1 _zero of_0;
+    of_0 <- aux_2;
+    x1 <- aux_1;
+    leakages <- LeakAddr([]) :: leakages;
+    aux_1 <- x1;
+    leakages <- LeakAddr([(4 + kk)]) :: leakages;
+    r.[(4 + kk)] <- aux_1;
+    return (_zero, of_0, cf, r);
+  }
+  
+  proc bn_muln (a:W64.t Array4.t, b:W64.t Array4.t) : W64.t * bool * bool *
+                                                      W64.t Array8.t = {
+    var aux_1: bool;
+    var aux_0: bool;
+    var aux_3: int;
+    var aux: W64.t;
+    var aux_2: W64.t Array8.t;
+    
+    var _zero:W64.t;
+    var of_0:bool;
+    var cf:bool;
+    var r:W64.t Array8.t;
+    var ai:W64.t;
+    var i:int;
+    var z:W64.t;
+    r <- witness;
+    leakages <- LeakAddr([0]) :: leakages;
+    aux <- a.[0];
+    ai <- aux;
+    leakages <- LeakAddr([]) :: leakages;
+    (aux, aux_1, aux_0, aux_2) <@ mul1 (ai, b);
+    _zero <- aux;
+    of_0 <- aux_1;
+    cf <- aux_0;
+    r <- aux_2;
+    leakages <- LeakFor(1,4) :: LeakAddr([]) :: leakages;
+    i <- 1;
+    while (i < 4) {
+      leakages <- LeakAddr([i]) :: leakages;
+      aux <- a.[i];
+      ai <- aux;
+      leakages <- LeakAddr([]) :: leakages;
+      aux <- (W64.of_int i);
+      z <- aux;
+      leakages <- LeakAddr([]) :: leakages;
+      (aux, aux_1, aux_0, aux_2) <@ mul1acc (z, ai, b, r, _zero, of_0, cf);
+      _zero <- aux;
+      of_0 <- aux_1;
+      cf <- aux_0;
+      r <- aux_2;
+      i <- i + 1;
+    }
+    return (_zero, of_0, cf, r);
+  }
+  
+  proc dmul1 (a:W64.t, b:W64.t Array8.t) : W64.t * bool * bool *
+                                           W64.t Array16.t = {
+    var aux_3: bool;
+    var aux_2: bool;
+    var aux_1: bool;
+    var aux_0: bool;
+    var aux: bool;
+    var aux_6: int;
+    var aux_5: W64.t;
+    var aux_4: W64.t;
+    
+    var _zero:W64.t;
+    var of_0:bool;
+    var cf:bool;
+    var r:W64.t Array16.t;
+    var x1:W64.t;
+    var x2:W64.t;
+    var i:int;
+    var lo:W64.t;
+    var  _0:bool;
+    var  _1:bool;
+    var  _2:bool;
+    r <- witness;
+    leakages <- LeakAddr([]) :: leakages;
+    (aux_3, aux_2, aux_1, aux_0, aux, aux_5) <- set0_64 ;
+    of_0 <- aux_3;
+    cf <- aux_2;
+     _0 <- aux_1;
+     _1 <- aux_0;
+     _2 <- aux;
+    _zero <- aux_5;
+    leakages <- LeakAddr([]) :: leakages;
+    aux_5 <- a;
+    x1 <- aux_5;
+    leakages <- LeakAddr([0]) :: leakages;
+    aux_5 <- b.[0];
+    x2 <- aux_5;
+    leakages <- LeakAddr([]) :: leakages;
+    (aux_5, aux_4) <- MULX_64 x1 x2;
+    x1 <- aux_5;
+    x2 <- aux_4;
+    leakages <- LeakAddr([]) :: leakages;
+    aux_5 <- x1;
+    leakages <- LeakAddr([1]) :: leakages;
+    r.[1] <- aux_5;
+    leakages <- LeakAddr([]) :: leakages;
+    aux_5 <- x2;
+    leakages <- LeakAddr([0]) :: leakages;
+    r.[0] <- aux_5;
+    leakages <- LeakFor(1,8) :: LeakAddr([]) :: leakages;
+    i <- 1;
+    while (i < 8) {
+      leakages <- LeakAddr([]) :: leakages;
+      aux_5 <- a;
+      x1 <- aux_5;
+      leakages <- LeakAddr([i]) :: leakages;
+      aux_5 <- b.[i];
+      x2 <- aux_5;
+      leakages <- LeakAddr([]) :: leakages;
+      (aux_5, aux_4) <- MULX_64 x1 x2;
+      x1 <- aux_5;
+      x2 <- aux_4;
+      leakages <- LeakAddr([]) :: leakages;
+      aux_5 <- x1;
+      leakages <- LeakAddr([(i + 1)]) :: leakages;
+      r.[(i + 1)] <- aux_5;
+      leakages <- LeakAddr([]) :: leakages;
+      aux_5 <- x2;
+      lo <- aux_5;
+      leakages <- LeakAddr([i]) :: leakages;
+      aux_5 <- r.[i];
+      x1 <- aux_5;
+      leakages <- LeakAddr([]) :: leakages;
+      aux_5 <- lo;
+      x2 <- aux_5;
+      leakages <- LeakAddr([]) :: leakages;
+      (aux_3, aux_5) <- ADCX_64 x1 x2 cf;
+      cf <- aux_3;
+      x1 <- aux_5;
+      leakages <- LeakAddr([]) :: leakages;
+      aux_5 <- x1;
+      leakages <- LeakAddr([i]) :: leakages;
+      r.[i] <- aux_5;
+      i <- i + 1;
+    }
+    leakages <- LeakAddr([8]) :: leakages;
+    aux_5 <- r.[8];
+    x1 <- aux_5;
+    leakages <- LeakAddr([]) :: leakages;
+    (aux_3, aux_5) <- ADCX_64 x1 _zero cf;
+    cf <- aux_3;
+    x1 <- aux_5;
+    leakages <- LeakAddr([]) :: leakages;
+    aux_5 <- x1;
+    leakages <- LeakAddr([8]) :: leakages;
+    r.[8] <- aux_5;
+    return (_zero, of_0, cf, r);
+  }
+  
+  proc dmul1acc (k:W64.t, a:W64.t, b:W64.t Array8.t, r:W64.t Array16.t,
+                 _zero:W64.t, of_0:bool, cf:bool) : W64.t * bool * bool *
+                                                    W64.t Array16.t = {
+    var aux_2: bool;
+    var aux: int;
+    var aux_1: W64.t;
+    var aux_0: W64.t;
+    
+    var kk:int;
+    var x1:W64.t;
+    var i:int;
+    var x2:W64.t;
+    var hi:W64.t;
+    var lo:W64.t;
+    
+    leakages <- LeakAddr([]) :: leakages;
+    aux <- (W64.to_uint k);
+    kk <- aux;
+    leakages <- LeakFor(0,(8 - 1)) :: LeakAddr([]) :: leakages;
+    aux <- (8 - 1);
+    i <- 0;
+    while (i < aux) {
+      leakages <- LeakAddr([]) :: leakages;
+      aux_1 <- a;
+      x1 <- aux_1;
+      leakages <- LeakAddr([i]) :: leakages;
+      aux_1 <- b.[i];
+      x2 <- aux_1;
+      leakages <- LeakAddr([]) :: leakages;
+      (aux_1, aux_0) <- MULX_64 x1 x2;
+      x1 <- aux_1;
+      x2 <- aux_0;
+      leakages <- LeakAddr([]) :: leakages;
+      aux_1 <- x1;
+      hi <- aux_1;
+      leakages <- LeakAddr([]) :: leakages;
+      aux_1 <- x2;
+      lo <- aux_1;
+      leakages <- LeakAddr([(kk + i)]) :: leakages;
+      aux_1 <- r.[(kk + i)];
+      x1 <- aux_1;
+      leakages <- LeakAddr([]) :: leakages;
+      (aux_2, aux_1) <- ADOX_64 x1 lo of_0;
+      of_0 <- aux_2;
+      x1 <- aux_1;
+      leakages <- LeakAddr([]) :: leakages;
+      aux_1 <- x1;
+      leakages <- LeakAddr([(kk + i)]) :: leakages;
+      r.[(kk + i)] <- aux_1;
+      leakages <- LeakAddr([((kk + i) + 1)]) :: leakages;
+      aux_1 <- r.[((kk + i) + 1)];
+      x1 <- aux_1;
+      leakages <- LeakAddr([]) :: leakages;
+      (aux_2, aux_1) <- ADCX_64 x1 hi cf;
+      cf <- aux_2;
+      x1 <- aux_1;
+      leakages <- LeakAddr([]) :: leakages;
+      aux_1 <- x1;
+      leakages <- LeakAddr([((kk + i) + 1)]) :: leakages;
+      r.[((kk + i) + 1)] <- aux_1;
+      i <- i + 1;
+    }
+    leakages <- LeakAddr([]) :: leakages;
+    aux_1 <- a;
+    x1 <- aux_1;
+    leakages <- LeakAddr([(8 - 1)]) :: leakages;
+    aux_1 <- b.[(8 - 1)];
+    x2 <- aux_1;
+    leakages <- LeakAddr([]) :: leakages;
+    (aux_1, aux_0) <- MULX_64 x1 x2;
+    x1 <- aux_1;
+    x2 <- aux_0;
+    leakages <- LeakAddr([]) :: leakages;
+    aux_1 <- x1;
+    leakages <- LeakAddr([(8 + kk)]) :: leakages;
+    r.[(8 + kk)] <- aux_1;
+    leakages <- LeakAddr([]) :: leakages;
+    aux_1 <- x2;
+    lo <- aux_1;
+    leakages <- LeakAddr([((8 + kk) - 1)]) :: leakages;
+    aux_1 <- r.[((8 + kk) - 1)];
+    x1 <- aux_1;
+    leakages <- LeakAddr([]) :: leakages;
+    (aux_2, aux_1) <- ADOX_64 x1 lo of_0;
+    of_0 <- aux_2;
+    x1 <- aux_1;
+    leakages <- LeakAddr([]) :: leakages;
+    aux_1 <- x1;
+    leakages <- LeakAddr([((8 + kk) - 1)]) :: leakages;
+    r.[((8 + kk) - 1)] <- aux_1;
+    leakages <- LeakAddr([(8 + kk)]) :: leakages;
+    aux_1 <- r.[(8 + kk)];
+    x1 <- aux_1;
+    leakages <- LeakAddr([]) :: leakages;
+    (aux_2, aux_1) <- ADCX_64 x1 _zero cf;
+    cf <- aux_2;
+    x1 <- aux_1;
+    leakages <- LeakAddr([]) :: leakages;
+    aux_1 <- x1;
+    leakages <- LeakAddr([(8 + kk)]) :: leakages;
+    r.[(8 + kk)] <- aux_1;
+    leakages <- LeakAddr([(8 + kk)]) :: leakages;
+    aux_1 <- r.[(8 + kk)];
+    x1 <- aux_1;
+    leakages <- LeakAddr([]) :: leakages;
+    (aux_2, aux_1) <- ADOX_64 x1 _zero of_0;
+    of_0 <- aux_2;
+    x1 <- aux_1;
+    leakages <- LeakAddr([]) :: leakages;
+    aux_1 <- x1;
+    leakages <- LeakAddr([(8 + kk)]) :: leakages;
+    r.[(8 + kk)] <- aux_1;
+    return (_zero, of_0, cf, r);
+  }
+  
+  proc dbn_muln (a:W64.t Array8.t, b:W64.t Array8.t) : W64.t * bool * bool *
+                                                       W64.t Array16.t = {
+    var aux_1: bool;
+    var aux_0: bool;
+    var aux_3: int;
+    var aux: W64.t;
+    var aux_2: W64.t Array16.t;
+    
+    var _zero:W64.t;
+    var of_0:bool;
+    var cf:bool;
+    var r:W64.t Array16.t;
+    var ai:W64.t;
+    var i:int;
+    var z:W64.t;
+    r <- witness;
+    leakages <- LeakAddr([0]) :: leakages;
+    aux <- a.[0];
+    ai <- aux;
+    leakages <- LeakAddr([]) :: leakages;
+    (aux, aux_1, aux_0, aux_2) <@ dmul1 (ai, b);
+    _zero <- aux;
+    of_0 <- aux_1;
+    cf <- aux_0;
+    r <- aux_2;
+    leakages <- LeakFor(1,8) :: LeakAddr([]) :: leakages;
+    i <- 1;
+    while (i < 8) {
+      leakages <- LeakAddr([i]) :: leakages;
+      aux <- a.[i];
+      ai <- aux;
+      leakages <- LeakAddr([]) :: leakages;
+      aux <- (W64.of_int i);
+      z <- aux;
+      leakages <- LeakAddr([]) :: leakages;
+      (aux, aux_1, aux_0, aux_2) <@ dmul1acc (z, ai, b, r, _zero, of_0, cf);
+      _zero <- aux;
+      of_0 <- aux_1;
+      cf <- aux_0;
+      r <- aux_2;
+      i <- i + 1;
+    }
+    return (_zero, of_0, cf, r);
+  }
+  
+  proc swapr (x:W64.t Array4.t, y:W64.t Array4.t, swap_0:W64.t) : W64.t Array4.t *
+                                                                  W64.t Array4.t = {
     var aux_0: int;
     var aux: W64.t;
     
@@ -157,9 +669,9 @@ module M = {
     leakages <- LeakAddr([]) :: leakages;
     aux <- (swap_0 * (W64.of_int 18446744073709551615));
     mask <- aux;
-    leakages <- LeakFor(0,32) :: LeakAddr([]) :: leakages;
+    leakages <- LeakFor(0,4) :: LeakAddr([]) :: leakages;
     i <- 0;
-    while (i < 32) {
+    while (i < 4) {
       leakages <- LeakAddr([i]) :: leakages;
       aux <- x.[i];
       tmp1 <- aux;
@@ -212,7 +724,7 @@ module M = {
     return (bit);
   }
   
-  proc ith_bit (kk:W64.t Array32.t, ctr:W64.t) : W64.t = {
+  proc ith_bit (kk:W64.t Array4.t, ctr:W64.t) : W64.t = {
     var aux: W64.t;
     
     var bit:W64.t;
@@ -243,28 +755,28 @@ module M = {
     return (bit);
   }
   
-  proc cminusP (p:W64.t Array32.t, x:W64.t Array32.t) : W64.t Array32.t = {
+  proc dcminusP (p:W64.t Array8.t, x:W64.t Array8.t) : W64.t Array8.t = {
     var aux_0: bool;
     var aux_1: int;
     var aux_2: W64.t;
-    var aux: W64.t Array32.t;
+    var aux: W64.t Array8.t;
     
-    var z:W64.t Array32.t;
+    var z:W64.t Array8.t;
     var cf:bool;
     var i:int;
     var r1:W64.t;
     var r2:W64.t;
     z <- witness;
     leakages <- LeakAddr([]) :: leakages;
-    aux <@ bn_copy (x);
+    aux <@ dbn_copy (x);
     z <- aux;
     leakages <- LeakAddr([]) :: leakages;
-    (aux_0, aux) <@ bn_subc (z, p);
+    (aux_0, aux) <@ dbn_subc (z, p);
     cf <- aux_0;
     z <- aux;
-    leakages <- LeakFor(0,32) :: LeakAddr([]) :: leakages;
+    leakages <- LeakFor(0,8) :: LeakAddr([]) :: leakages;
     i <- 0;
-    while (i < 32) {
+    while (i < 8) {
       leakages <- LeakAddr([i]) :: leakages;
       aux_2 <- z.[i];
       r1 <- aux_2;
@@ -283,47 +795,196 @@ module M = {
     return (x);
   }
   
-  proc addm (p:W64.t Array32.t, a:W64.t Array32.t, b:W64.t Array32.t) : 
-  W64.t Array32.t = {
-    var aux: bool;
-    var aux_0: W64.t Array32.t;
+  proc bn_expand (x:W64.t Array4.t) : W64.t Array8.t = {
+    var aux: int;
+    var aux_0: W64.t;
     
-    var  _0:bool;
+    var r:W64.t Array8.t;
+    var i:int;
+    r <- witness;
+    leakages <- LeakFor(0,4) :: LeakAddr([]) :: leakages;
+    i <- 0;
+    while (i < 4) {
+      leakages <- LeakAddr([i]) :: leakages;
+      aux_0 <- x.[i];
+      leakages <- LeakAddr([i]) :: leakages;
+      r.[i] <- aux_0;
+      i <- i + 1;
+    }
+    leakages <- LeakFor(4,8) :: LeakAddr([]) :: leakages;
+    i <- 4;
+    while (i < 8) {
+      leakages <- LeakAddr([]) :: leakages;
+      aux_0 <- (W64.of_int 0);
+      leakages <- LeakAddr([i]) :: leakages;
+      r.[i] <- aux_0;
+      i <- i + 1;
+    }
+    return (r);
+  }
+  
+  proc bn_shrink (x:W64.t Array8.t) : W64.t Array4.t = {
+    var aux: int;
+    var aux_0: W64.t;
     
+    var r:W64.t Array4.t;
+    var i:int;
+    r <- witness;
+    leakages <- LeakFor(0,4) :: LeakAddr([]) :: leakages;
+    i <- 0;
+    while (i < 4) {
+      leakages <- LeakAddr([i]) :: leakages;
+      aux_0 <- x.[i];
+      leakages <- LeakAddr([i]) :: leakages;
+      r.[i] <- aux_0;
+      i <- i + 1;
+    }
+    return (r);
+  }
+  
+  proc div2 (x:W64.t Array16.t, k:int) : W64.t Array8.t = {
+    var aux: int;
+    var aux_0: W64.t;
+    
+    var r:W64.t Array8.t;
+    var i:int;
+    r <- witness;
+    leakages <- LeakFor(0,k) :: LeakAddr([]) :: leakages;
+    aux <- k;
+    i <- 0;
+    while (i < aux) {
+      leakages <- LeakAddr([(8 + i)]) :: leakages;
+      aux_0 <- x.[(8 + i)];
+      leakages <- LeakAddr([i]) :: leakages;
+      r.[i] <- aux_0;
+      i <- i + 1;
+    }
+    return (r);
+  }
+  
+  proc bnreduce (a:W64.t Array8.t, r:W64.t Array8.t, p:W64.t Array4.t) : 
+  W64.t Array4.t = {
+    var aux_1: bool;
+    var aux_0: bool;
+    var aux: W64.t;
+    var aux_4: W64.t Array4.t;
+    var aux_3: W64.t Array8.t;
+    var aux_2: W64.t Array16.t;
+    
+    var res_0:W64.t Array4.t;
+    var xr:W64.t Array16.t;
+    var xrf:W64.t Array8.t;
+    var xrfd:W64.t Array4.t;
+    var xrfn:W64.t Array8.t;
+    var t:W64.t Array8.t;
+    var pp:W64.t Array8.t;
+    var  _0:W64.t;
+    var  _1:bool;
+    var  _2:bool;
+    var  _3:W64.t;
+    var  _4:bool;
+    var  _5:bool;
+    var  _6:bool;
+    pp <- witness;
+    res_0 <- witness;
+    t <- witness;
+    xr <- witness;
+    xrf <- witness;
+    xrfd <- witness;
+    xrfn <- witness;
     leakages <- LeakAddr([]) :: leakages;
-    (aux, aux_0) <@ bn_addc (a, b);
+    (aux, aux_1, aux_0, aux_2) <@ dbn_muln (a, r);
      _0 <- aux;
-    a <- aux_0;
+     _1 <- aux_1;
+     _2 <- aux_0;
+    xr <- aux_2;
     leakages <- LeakAddr([]) :: leakages;
-    aux_0 <@ cminusP (p, a);
-    a <- aux_0;
+    aux_3 <@ div2 (xr, (2 * 4));
+    xrf <- aux_3;
+    leakages <- LeakAddr([]) :: leakages;
+    aux_4 <@ bn_shrink (xrf);
+    xrfd <- aux_4;
+    leakages <- LeakAddr([]) :: leakages;
+    (aux, aux_1, aux_0, aux_3) <@ bn_muln (xrfd, p);
+     _3 <- aux;
+     _4 <- aux_1;
+     _5 <- aux_0;
+    xrfn <- aux_3;
+    leakages <- LeakAddr([]) :: leakages;
+    (aux_1, aux_3) <@ dbn_subc (a, xrfn);
+     _6 <- aux_1;
+    t <- aux_3;
+    leakages <- LeakAddr([]) :: leakages;
+    aux_3 <@ bn_expand (p);
+    pp <- aux_3;
+    leakages <- LeakAddr([]) :: leakages;
+    aux_3 <@ dcminusP (pp, t);
+    t <- aux_3;
+    leakages <- LeakAddr([]) :: leakages;
+    aux_4 <@ bn_shrink (t);
+    res_0 <- aux_4;
+    return (res_0);
+  }
+  
+  proc mulmr (p:W64.t Array4.t, a:W64.t Array4.t, b:W64.t Array4.t) : 
+  W64.t Array4.t = {
+    var aux_2: bool;
+    var aux_1: bool;
+    var aux_0: W64.t;
+    var aux_3: W64.t Array4.t;
+    var aux: W64.t Array8.t;
+    
+    var d:W64.t Array8.t;
+    var _of:bool;
+    var _cf:bool;
+    var c:W64.t Array8.t;
+    var  _0:W64.t;
+    c <- witness;
+    d <- witness;
+    leakages <- LeakAddr([]) :: leakages;
+    aux <@ bn2_set0 (d);
+    d <- aux;
+    leakages <- LeakAddr([]) :: leakages;
+    aux_0 <- (W64.of_int 4);
+    leakages <- LeakAddr([0]) :: leakages;
+    d.[0] <- aux_0;
+    leakages <- LeakAddr([]) :: leakages;
+    (aux_0, aux_2, aux_1, aux) <@ bn_muln (a, b);
+     _0 <- aux_0;
+    _of <- aux_2;
+    _cf <- aux_1;
+    c <- aux;
+    leakages <- LeakAddr([]) :: leakages;
+    aux_3 <@ bnreduce (c, d, p);
+    a <- aux_3;
     return (a);
   }
   
-  proc mulm (m:W64.t Array32.t, x:W64.t Array32.t, n:W64.t Array32.t) : 
-  W64.t Array32.t = {
+  proc expm (m:W64.t Array4.t, x:W64.t Array4.t, n:W64.t Array4.t) : 
+  W64.t Array4.t = {
     var aux: W64.t;
-    var aux_1: W64.t Array32.t;
-    var aux_0: W64.t Array32.t;
+    var aux_1: W64.t Array4.t;
+    var aux_0: W64.t Array4.t;
     
-    var x1:W64.t Array32.t;
+    var x1:W64.t Array4.t;
     var ctr:W64.t;
-    var x2:W64.t Array32.t;
+    var x2:W64.t Array4.t;
     var d:W64.t;
-    var x3:W64.t Array32.t;
-    var x4:W64.t Array32.t;
+    var x3:W64.t Array4.t;
+    var x4:W64.t Array4.t;
     var p:W64.t;
     var lbit:W64.t;
     var t1:W64.t;
     var t2:W64.t;
-    var q:W64.t;
     var par:W64.t;
+    var q:W64.t;
+    var cbit:W64.t;
     x1 <- witness;
     x2 <- witness;
     x3 <- witness;
     x4 <- witness;
     leakages <- LeakAddr([]) :: leakages;
-    aux <- (W64.of_int ((32 * 64) - 1));
+    aux <- (W64.of_int ((4 * 64) - 1));
     ctr <- aux;
     leakages <- LeakAddr([]) :: leakages;
     aux_1 <@ bn_set0 (x1);
@@ -338,7 +999,7 @@ module M = {
     aux_1 <@ bn_copy (x);
     x3 <- aux_1;
     leakages <- LeakAddr([]) :: leakages;
-    aux_1 <@ addm (m, x, x);
+    aux_1 <@ mulmr (m, x, x3);
     x4 <- aux_1;
     leakages <- LeakAddr([]) :: leakages;
     aux <- d;
@@ -371,9 +1032,6 @@ module M = {
       aux <- d;
       p <- aux;
       leakages <- LeakAddr([]) :: leakages;
-      aux <- d;
-      q <- aux;
-      leakages <- LeakAddr([]) :: leakages;
       aux <- (d `|` t2);
       d <- aux;
       leakages <- LeakAddr([]) :: leakages;
@@ -384,50 +1042,52 @@ module M = {
       x1 <- aux_1;
       x2 <- aux_0;
       leakages <- LeakAddr([]) :: leakages;
-      aux_1 <@ addm (m, x1, x2);
+      aux_1 <@ mulmr (m, x1, x2);
       x1 <- aux_1;
+      leakages <- LeakAddr([]) :: leakages;
+      aux_1 <@ mulmr (m, x2, x2);
+      x2 <- aux_1;
+      leakages <- LeakAddr([]) :: leakages;
+      aux <- d;
+      q <- aux;
+      leakages <- LeakAddr([]) :: leakages;
+      aux <- (q `^` p);
+      cbit <- aux;
+      leakages <- LeakAddr([]) :: leakages;
+      (aux_1, aux_0) <@ swapr (x1, x3, cbit);
+      x1 <- aux_1;
+      x3 <- aux_0;
+      leakages <- LeakAddr([]) :: leakages;
+      (aux_1, aux_0) <@ swapr (x2, x4, cbit);
+      x2 <- aux_1;
+      x4 <- aux_0;
     leakages <- LeakCond(((W64.of_int 0) \ult ctr)) :: LeakAddr([]) :: leakages;
     
     }
     leakages <- LeakAddr([]) :: leakages;
     aux <@ ith_bit (n, (W64.of_int 0));
-    par <- aux;
+    p <- aux;
     leakages <- LeakAddr([]) :: leakages;
-    (aux_1, aux_0) <@ swapr (x2, x1, par);
+    (aux_1, aux_0) <@ swapr (x2, x1, p);
     x1 <- aux_1;
     x2 <- aux_0;
     return (x1);
   }
   
   proc toEC () : unit = {
-    var aux_0: W64.t;
-    var aux_1: W64.t Array32.t;
-    var aux: W64.t Array32.t;
+    var aux: W64.t Array4.t;
     
-    var p:W64.t Array32.t;
-    var a:W64.t Array32.t;
-    var b:W64.t Array32.t;
-    var r:W64.t Array32.t;
-    var x:W64.t;
-    var  _0:W64.t Array32.t;
-     _0 <- witness;
+    var a:W64.t Array4.t;
+    var b:W64.t Array4.t;
+    var p:W64.t Array4.t;
+    var r:W64.t Array4.t;
     a <- witness;
     b <- witness;
     p <- witness;
     r <- witness;
     leakages <- LeakAddr([]) :: leakages;
-    aux_1 <@ addm (p, a, b);
-    r <- aux_1;
-    leakages <- LeakAddr([]) :: leakages;
-    aux_1 <@ mulm (p, a, b);
-    r <- aux_1;
-    leakages <- LeakAddr([]) :: leakages;
-    aux_0 <@ ith_bit (a, x);
-    x <- aux_0;
-    leakages <- LeakAddr([]) :: leakages;
-    (aux_1, aux) <@ swapr (a, a, x);
-     _0 <- aux_1;
-    a <- aux;
+    aux <@ expm (a, b, p);
+    r <- aux;
     return ();
   }
 }.
