w64x4/proof/Fp_w64x4_extract.ec
@@ -1,5 +1,5 @@
 require import AllCore IntDiv CoreMap List Distr.
- require import JModel.
+(* from Jasmin *) require import JModel.
 
 require import Array4 Array8 Array16.
 (* require import WArray32 WArray64 WArray128. *)
@@ -30,6 +30,22 @@ module M = {
     return (cf, a);
   }
   
+  proc bn_copy (a:W64.t Array4.t) : W64.t Array4.t = {
+    var aux: int;
+    
+    var r:W64.t Array4.t;
+    var i:int;
+    var t:W64.t;
+    r <- witness;
+    i <- 0;
+    while (i < 4) {
+      t <- a.[i];
+      r.[i] <- t;
+      i <- i + 1;
+    }
+    return (r);
+  }
+  
   proc dbn_copy (a:W64.t Array8.t) : W64.t Array8.t = {
     var aux: int;
     
@@ -44,6 +60,33 @@ module M = {
       i <- i + 1;
     }
     return (r);
+  }
+  
+  proc bn_set0 (a:W64.t Array4.t) : W64.t Array4.t = {
+    var aux: int;
+    
+    var i:int;
+    
+    i <- 0;
+    while (i < 4) {
+      a.[i] <- (W64.of_int 0);
+      i <- i + 1;
+    }
+    return (a);
+  }
+  
+  proc bn2_set0 (a:W64.t Array8.t) : W64.t Array8.t = {
+    var aux: int;
+    
+    var i:int;
+    
+    aux <- (2 * 4);
+    i <- 0;
+    while (i < aux) {
+      a.[i] <- (W64.of_int 0);
+      i <- i + 1;
+    }
+    return (a);
   }
   
   proc mul1 (a:W64.t, b:W64.t Array4.t) : W64.t * bool * bool *
@@ -87,17 +130,19 @@ module M = {
     return (_zero, of_0, cf, r);
   }
   
-  proc mul1acc (k:int, a:W64.t, b:W64.t Array4.t, r:W64.t Array8.t,
+  proc mul1acc (k:W64.t, a:W64.t, b:W64.t Array4.t, r:W64.t Array8.t,
                 _zero:W64.t, of_0:bool, cf:bool) : W64.t * bool * bool *
                                                    W64.t Array8.t = {
     var aux: int;
     
+    var kk:int;
     var x1:W64.t;
     var i:int;
     var x2:W64.t;
     var hi:W64.t;
     var lo:W64.t;
     
+    kk <- (W64.to_uint k);
     aux <- (4 - 1);
     i <- 0;
     while (i < aux) {
@@ -106,28 +151,28 @@ module M = {
       (x1, x2) <- MULX_64 x1 x2;
       hi <- x1;
       lo <- x2;
-      x1 <- r.[(k + i)];
+      x1 <- r.[(kk + i)];
       (of_0, x1) <- ADOX_64 x1 lo of_0;
-      r.[(k + i)] <- x1;
-      x1 <- r.[((k + i) + 1)];
+      r.[(kk + i)] <- x1;
+      x1 <- r.[((kk + i) + 1)];
       (cf, x1) <- ADCX_64 x1 hi cf;
-      r.[((k + i) + 1)] <- x1;
+      r.[((kk + i) + 1)] <- x1;
       i <- i + 1;
     }
     x1 <- a;
     x2 <- b.[(4 - 1)];
     (x1, x2) <- MULX_64 x1 x2;
-    r.[(4 + k)] <- x1;
+    r.[(4 + kk)] <- x1;
     lo <- x2;
-    x1 <- r.[((4 + k) - 1)];
+    x1 <- r.[((4 + kk) - 1)];
     (of_0, x1) <- ADOX_64 x1 lo of_0;
-    r.[((4 + k) - 1)] <- x1;
-    x1 <- r.[(4 + k)];
+    r.[((4 + kk) - 1)] <- x1;
+    x1 <- r.[(4 + kk)];
     (cf, x1) <- ADCX_64 x1 _zero cf;
-    r.[(4 + k)] <- x1;
-    x1 <- r.[(4 + k)];
+    r.[(4 + kk)] <- x1;
+    x1 <- r.[(4 + kk)];
     (of_0, x1) <- ADOX_64 x1 _zero of_0;
-    r.[(4 + k)] <- x1;
+    r.[(4 + kk)] <- x1;
     return (_zero, of_0, cf, r);
   }
   
@@ -141,13 +186,15 @@ module M = {
     var r:W64.t Array8.t;
     var ai:W64.t;
     var i:int;
+    var z:W64.t;
     r <- witness;
     ai <- a.[0];
     (_zero, of_0, cf, r) <@ mul1 (ai, b);
     i <- 1;
     while (i < 4) {
       ai <- a.[i];
-      (_zero, of_0, cf, r) <@ mul1acc (i, ai, b, r, _zero, of_0, cf);
+      z <- (W64.of_int i);
+      (_zero, of_0, cf, r) <@ mul1acc (z, ai, b, r, _zero, of_0, cf);
       i <- i + 1;
     }
     return (_zero, of_0, cf, r);
@@ -194,17 +241,19 @@ module M = {
     return (_zero, of_0, cf, r);
   }
   
-  proc dmul1acc (k:int, a:W64.t, b:W64.t Array8.t, r:W64.t Array16.t,
+  proc dmul1acc (k:W64.t, a:W64.t, b:W64.t Array8.t, r:W64.t Array16.t,
                  _zero:W64.t, of_0:bool, cf:bool) : W64.t * bool * bool *
                                                     W64.t Array16.t = {
     var aux: int;
     
+    var kk:int;
     var x1:W64.t;
     var i:int;
     var x2:W64.t;
     var hi:W64.t;
     var lo:W64.t;
     
+    kk <- (W64.to_uint k);
     aux <- (8 - 1);
     i <- 0;
     while (i < aux) {
@@ -213,28 +262,28 @@ module M = {
       (x1, x2) <- MULX_64 x1 x2;
       hi <- x1;
       lo <- x2;
-      x1 <- r.[(k + i)];
+      x1 <- r.[(kk + i)];
       (of_0, x1) <- ADOX_64 x1 lo of_0;
-      r.[(k + i)] <- x1;
-      x1 <- r.[((k + i) + 1)];
+      r.[(kk + i)] <- x1;
+      x1 <- r.[((kk + i) + 1)];
       (cf, x1) <- ADCX_64 x1 hi cf;
-      r.[((k + i) + 1)] <- x1;
+      r.[((kk + i) + 1)] <- x1;
       i <- i + 1;
     }
     x1 <- a;
     x2 <- b.[(8 - 1)];
     (x1, x2) <- MULX_64 x1 x2;
-    r.[(8 + k)] <- x1;
+    r.[(8 + kk)] <- x1;
     lo <- x2;
-    x1 <- r.[((8 + k) - 1)];
+    x1 <- r.[((8 + kk) - 1)];
     (of_0, x1) <- ADOX_64 x1 lo of_0;
-    r.[((8 + k) - 1)] <- x1;
-    x1 <- r.[(8 + k)];
+    r.[((8 + kk) - 1)] <- x1;
+    x1 <- r.[(8 + kk)];
     (cf, x1) <- ADCX_64 x1 _zero cf;
-    r.[(8 + k)] <- x1;
-    x1 <- r.[(8 + k)];
+    r.[(8 + kk)] <- x1;
+    x1 <- r.[(8 + kk)];
     (of_0, x1) <- ADOX_64 x1 _zero of_0;
-    r.[(8 + k)] <- x1;
+    r.[(8 + kk)] <- x1;
     return (_zero, of_0, cf, r);
   }
   
@@ -248,16 +297,73 @@ module M = {
     var r:W64.t Array16.t;
     var ai:W64.t;
     var i:int;
+    var z:W64.t;
     r <- witness;
     ai <- a.[0];
     (_zero, of_0, cf, r) <@ dmul1 (ai, b);
     i <- 1;
     while (i < 8) {
       ai <- a.[i];
-      (_zero, of_0, cf, r) <@ dmul1acc (i, ai, b, r, _zero, of_0, cf);
+      z <- (W64.of_int i);
+      (_zero, of_0, cf, r) <@ dmul1acc (z, ai, b, r, _zero, of_0, cf);
       i <- i + 1;
     }
     return (_zero, of_0, cf, r);
+  }
+  
+  proc swapr (x:W64.t Array4.t, y:W64.t Array4.t, swap_0:W64.t) : W64.t Array4.t *
+                                                                  W64.t Array4.t = {
+    var aux: int;
+    
+    var mask:W64.t;
+    var i:int;
+    var tmp1:W64.t;
+    var tmp2:W64.t;
+    
+    mask <- (swap_0 * (W64.of_int 18446744073709551615));
+    i <- 0;
+    while (i < 4) {
+      tmp1 <- x.[i];
+      tmp1 <- (tmp1 `^` y.[i]);
+      tmp1 <- (tmp1 `&` mask);
+      x.[i] <- (x.[i] `^` tmp1);
+      tmp2 <- y.[i];
+      tmp2 <- (tmp2 `^` tmp1);
+      y.[i] <- tmp2;
+      i <- i + 1;
+    }
+    return (x, y);
+  }
+  
+  proc ith_bit64 (k:W64.t, ctr:W64.t) : W64.t = {
+    
+    var bit:W64.t;
+    var p:W64.t;
+    
+    bit <- k;
+    p <- ctr;
+    p <- (p `&` (W64.of_int 63));
+    bit <- (bit `>>` (truncateu8 p));
+    bit <- (bit `&` (W64.of_int 1));
+    return (bit);
+  }
+  
+  proc ith_bit (kk:W64.t Array4.t, ctr:W64.t) : W64.t = {
+    
+    var bit:W64.t;
+    var ctr2:W64.t;
+    var ctr3:W64.t;
+    var c1:W64.t;
+    var c2:W64.t;
+    var r:W64.t;
+    
+    ctr2 <- ctr;
+    ctr3 <- ctr;
+    c1 <- (ctr2 `>>` (W8.of_int 6));
+    c2 <- (ctr3 `&` (W64.of_int 63));
+    r <- kk.[(W64.to_uint c1)];
+    bit <@ ith_bit64 (r, c2);
+    return (bit);
   }
   
   proc dcminusP (p:W64.t Array8.t, x:W64.t Array8.t) : W64.t Array8.t = {
@@ -365,15 +471,85 @@ module M = {
     return (res_0);
   }
   
+  proc mulmr (p:W64.t Array4.t, a:W64.t Array4.t, b:W64.t Array4.t) : 
+  W64.t Array4.t = {
+    
+    var d:W64.t Array8.t;
+    var _of:bool;
+    var _cf:bool;
+    var c:W64.t Array8.t;
+    var  _0:W64.t;
+    c <- witness;
+    d <- witness;
+    d <@ bn2_set0 (d);
+    d.[0] <- (W64.of_int 4);
+    ( _0, _of, _cf, c) <@ bn_muln (a, b);
+    a <@ bnreduce (c, d, p);
+    return (a);
+  }
+  
+  proc expm (m:W64.t Array4.t, x:W64.t Array4.t, n:W64.t Array4.t) : 
+  W64.t Array4.t = {
+    
+    var x1:W64.t Array4.t;
+    var ctr:W64.t;
+    var x2:W64.t Array4.t;
+    var d:W64.t;
+    var x3:W64.t Array4.t;
+    var x4:W64.t Array4.t;
+    var p:W64.t;
+    var lbit:W64.t;
+    var t1:W64.t;
+    var t2:W64.t;
+    var par:W64.t;
+    var q:W64.t;
+    var cbit:W64.t;
+    x1 <- witness;
+    x2 <- witness;
+    x3 <- witness;
+    x4 <- witness;
+    ctr <- (W64.of_int ((4 * 64) - 1));
+    x1 <@ bn_set0 (x1);
+    x2 <@ bn_set0 (x2);
+    d <@ ith_bit (n, ctr);
+    x3 <@ bn_copy (x);
+    x4 <@ mulmr (m, x, x3);
+    p <- d;
+    (x1, x3) <@ swapr (x1, x3, d);
+    (x2, x4) <@ swapr (x2, x4, d);
+    
+    while (((W64.of_int 0) \ult ctr)) {
+      lbit <- ctr;
+      ctr <- (ctr - (W64.of_int 1));
+      t1 <@ ith_bit (n, lbit);
+      t2 <@ ith_bit (n, ctr);
+      p <- d;
+      d <- (d `|` t2);
+      par <- (t1 `^` t2);
+      (x1, x2) <@ swapr (x1, x2, par);
+      x1 <@ mulmr (m, x1, x2);
+      x2 <@ mulmr (m, x2, x2);
+      q <- d;
+      cbit <- (q `^` p);
+      (x1, x3) <@ swapr (x1, x3, cbit);
+      (x2, x4) <@ swapr (x2, x4, cbit);
+    }
+    p <@ ith_bit (n, (W64.of_int 0));
+    (x1, x2) <@ swapr (x2, x1, p);
+    return (x1);
+  }
+  
   proc toEC () : unit = {
     
-    var z:W64.t Array8.t;
+    var a:W64.t Array4.t;
+    var b:W64.t Array4.t;
     var p:W64.t Array4.t;
     var r:W64.t Array4.t;
+    a <- witness;
+    b <- witness;
     p <- witness;
     r <- witness;
-    z <- witness;
-    r <@ bnreduce (z, z, p);
+    r <@ expm (a, b, p);
     return ();
   }
 }.
