w64x4/proof/Fp_w64x4_proof_mulm.ec
@@ -10,6 +10,8 @@ require import Ith_Bit64.
 import Array16 Array8 Array4.
 import Zp W64x4 R.
 
+import StdBigop Bigint BIA.
+
 
 equiv mul1first_eq:
  M.mul1 ~ MulOps.mul1:
@@ -24,18 +26,20 @@ while ( #pre /\ ={r,i} /\ (a,of_0,cf,_zero){1}=(ak,_of,_cf,W64.zero){2} /\
  wp; skip => />; smt(Array8.get_setE Array8.set_set_if).
 wp; skip => />; smt (Array8.set_set_if).
 qed.
+
+
 equiv mul1acc_eq :
  M.mul1acc ~ MulOps.mul1acc:
- ={k,a,b} /\ (_zero,of_0,cf,r){1}=(W64.zero,_of,_cf,x){2} /\
+ W64.to_uint k{1} = k{2} /\ ={a,b} /\ (_zero,of_0,cf,r){1}=(W64.zero,_of,_cf,x){2} /\
   0 <= k{2} < nlimbs
  ==>
  (res.`1,res.`2,res.`3,res.`4){1} = (W64.zero,res.`1,res.`2,res.`3){2}.
 proof.
 proc. simplify.
 wp. while ( #pre /\ ={i} /\ (aux,_zero){1}=(nlimbs-1,W64.zero){2} /\ 
-            0 <= i{2} <= nlimbs-1).
- wp; skip => />; smt(get_setE set_set_if).
-wp; skip; smt(get_setE set_set_if).
+            0 <= i{2} <= nlimbs-1 /\ kk{1} = k{2}).
+ wp; skip => />; smt(Array8.get_setE Array8.set_set_if).
+wp; skip; smt(Array8.get_setE Array8.set_set_if).
 qed.
 
 
@@ -48,30 +52,33 @@ proof.
 proc; simplify.
 wp.
 while ( #pre /\ ={r,i} /\ (a,of_0,cf,_zero){1}=(ak,_of,_cf,W64.zero){2} /\ 
-        1 <= i{2} <= 8 /\ !_of{2}).
+        1 <= i{2} <= dnlimbs /\ !_of{2}).
  wp; skip => />; smt(Array16.get_setE Array16.set_set_if).
 wp; skip => />; smt (Array16.set_set_if).
 qed.
+
+
 equiv dmul1acc_eq :
  M.dmul1acc ~ W64x8.MulOps.mul1acc:
- ={k,a,b} /\ (_zero,of_0,cf,r){1}=(W64.zero,_of,_cf,x){2} /\
-  0 <= k{2} < 8
+   W64.to_uint k{1} = k{2} /\ ={a,b} /\ (_zero,of_0,cf,r){1}=(W64.zero,_of,_cf,x){2} /\
+  0 <= k{2} < dnlimbs
  ==>
  (res.`1,res.`2,res.`3,res.`4){1} = (W64.zero,res.`1,res.`2,res.`3){2}.
 proof.
 proc. simplify.
 wp. while ( #pre /\ ={i} /\ (aux,_zero){1}=(8-1,W64.zero){2} /\ 
-            0 <= i{2} <= 8-1).
- wp; skip => />; smt(get_setE set_set_if).
-wp; skip; smt(get_setE set_set_if).
+            0 <= i{2} <= 8-1 /\ kk{1} = k{2}).
+ wp; skip => />; smt(Array16.get_setE Array16.set_set_if).
+wp; skip; smt(Array16.get_setE Array16.set_set_if).
 qed.
 
 
 equiv muln_spec:
  M.bn_muln ~ ASpecFp.muln:
   ImplZZ a{1} a{2} /\ ImplZZ b{1} b{2}
-  ==> ImplZZ2 res{1}.`4 res{2}
-      /\ res{1}.`1 = W64.zero /\ !res{1}.`2 /\ !res{1}.`3.
+  ==> 
+  ImplZZ2 res{1}.`4 res{2}
+     /\ res{1}.`1 = W64.zero /\ !res{1}.`2 /\ !res{1}.`3.
 proof.
 transitivity 
  MulOps.mulR
@@ -83,7 +90,8 @@ transitivity
 + proc; simplify.
   while ( #pre /\ (i,_zero,of_0,cf,r){1}=(k,W64.zero,_of,_cf,r){2} /\
           1 <= k{2} <= nlimbs ).
-   by wp; call mul1acc_eq; wp; skip => /> /#.
+  wp. call mul1acc_eq. wp. skip. smt.
+   (* by wp; call mul1acc_eq; wp; skip => /> /#. *)
   by wp; call mul1first_eq; wp; skip => /> /#.
 + proc.
   transitivity {1}
@@ -97,12 +105,12 @@ transitivity
 qed.
 
 
-
 equiv dmuln_spec:
  M.dbn_muln ~ ASpecFp.muln:
   W64x8.valR a{1} = a{2} /\  W64x8.valR b{1} = b{2}
-  ==> W64x8.valR2 res{1}.`4 = res{2}
-      /\ res{1}.`1 = W64.zero /\ !res{1}.`2 /\ !res{1}.`3.
+  ==> 
+ W64x8.valR2 res{1}.`4 = res{2}
+     /\ res{1}.`1 = W64.zero /\ !res{1}.`2 /\ !res{1}.`3.
 proof.
 transitivity 
  W64x8.MulOps.mulR
@@ -113,8 +121,9 @@ transitivity
 + by move=> /> /#.
 + proc; simplify.
   while ( #pre /\ (i,_zero,of_0,cf,r){1}=(k,W64.zero,_of,_cf,r){2} /\
-          1 <= k{2} <= 8 ).
-   by wp; call dmul1acc_eq; wp; skip => /> /#.
+          1 <= k{2} <= dnlimbs ).
+  wp. call dmul1acc_eq. wp. skip. smt.
+   (* by wp; call dmul1acc_eq; wp; skip => /> /#;smt. *)
   by wp; call dmul1first_eq; wp; skip => /> /#.
 + proc.
   transitivity {1}
@@ -126,9 +135,6 @@ transitivity
   + by inline W64x8.MulOps.mulR; sim.
   + by ecall {1} (W64x8.mulR_ph a{1} b{1}); wp; skip.
 qed.
-
-
-import W64x8.
 
 
 equiv dsubc_spec:
@@ -146,10 +152,10 @@ transitivity
 + proc; simplify.
   unroll {2} 3; rcondt {2} 3; first by auto.
   exlim a{1}, b{1} => aa bb.
-  while (={i,b} /\ 1 <= i{2} <= 8 /\ 
+  while (={i,b} /\ 1 <= i{2} <= dnlimbs /\ 
          (cf, aa){1}=(c, a){2} /\
          (forall k, 0 <= k < i{2} => a{1}.[k] = r{2}.[k])%Array8 /\
-         (forall k, i{2} <= k < 8 => a{1}.[k] = aa.[k])%Array8).
+         (forall k, i{2} <= k < dnlimbs => a{1}.[k] = aa.[k])%Array8).
    wp; skip => /> &1 &2 Hi1 _ Hh1 Hh2 Hi2.
    split => *; first smt().
    split => *; first smt().
@@ -181,7 +187,6 @@ transitivity
 progress. 
     by rewrite W64x8.R.bn_borrowE 1:/# b2i0 /bn_modulus /=.
 qed.
-
 
 
 
@@ -229,27 +234,26 @@ qed.
 
 
 
-import StdBigop.
-import Bigint.
-import BIA.
-lemma bn_div2_correct  z :
-  phoare[ M.div2 : arg = (z,2*nlimbs)  ==> (W64x8.valR res) = (W64x8.valR2 z) %/  2^(8*64) ] = 1%r.
+import W64x8.
+
+lemma bn_div2_correct z :
+  phoare[ M.div2 : arg = (z,dnlimbs)  ==> (W64x8.valR res) = (W64x8.valR2 z) %/  W64x8.modulusR ] = 1%r.
 proc. sp.
-while (aux = 2*nlimbs /\ i <= 2*nlimbs /\ forall j, 0 <= j < i => r.[j] = x.[2*nlimbs + j]) (2*nlimbs - i) . progress. wp. skip. progress.
+while (aux = dnlimbs /\ i <= dnlimbs /\ forall j, 0 <= j < i => r.[j] = x.[dnlimbs + j]) (dnlimbs - i) . progress. wp. skip. progress.
 smt. smt. smt. skip. progress.
 smt. smt.
-have ->: 13407807929942597099574024998205846127479365820592393377723561443721764030073546976801874298166903427690031858186486050853753882811946569946433649006084096 = W64x8.M^8. smt.
-have ->: (R2.bnk 16 x{hr})%R2 = valR2 x{hr}. auto.
+have -> :  W64x8.modulusR  = W64x8.M^dnlimbs.  rewrite /R.bn_modulus. auto. 
+have ->: (R2.bnk (2*dnlimbs) x{hr})%R2 = valR2 x{hr}. auto.
 rewrite R2.bghint_div. auto.
 rewrite - R.bnkup0.
 rewrite /bnkup.
 have ->: 
-  bigi predT (fun (i1 : int) => to_uint r0.[i1] * W64x8.M ^ (i1 - 0)) 0 8
-  = bigi predT (fun (i1 : int) => to_uint x{hr}.[i1 + 8] * W64x8.M ^ (i1 - 0)) 0 8.
+  bigi predT (fun (i1 : int) => to_uint r0.[i1] * W64x8.M ^ (i1 - 0)) 0 dnlimbs
+  = bigi predT (fun (i1 : int) => to_uint x{hr}.[i1 + dnlimbs] * W64x8.M ^ (i1 - 0)) 0 dnlimbs.
 apply eq_big_int. progress. smt. 
-  have ->: bigi predT (fun (i1 : int) => to_uint x{hr}.[i1] * W64x8.M ^ (i1 - 8)) 8
-  (2 * 8)  = bigi predT (fun (i1 : int) => to_uint x{hr}.[i1] * W64x8.M ^ (i1 - 8)) (0 + 8)
-  (2 * 8). auto.
+  have ->: bigi predT (fun (i1 : int) => to_uint x{hr}.[i1] * W64x8.M ^ (i1 - dnlimbs)) dnlimbs
+  (2 * dnlimbs)  = bigi predT (fun (i1 : int) => to_uint x{hr}.[i1] * W64x8.M ^ (i1 - dnlimbs)) (0 + dnlimbs)
+  (2 * dnlimbs). auto.
 rewrite big_addn. simplify. auto.
 qed.
 
@@ -264,74 +268,67 @@ while (i <= nlimbs /\ forall j, 0 <= j < i => r.[j]%Array4 = x.[j]%Array8) (nlim
 smt. smt. smt. skip. progress.
 progress. 
 smt. smt. 
-have ->: W64x4.modulusR = W64x8.M ^ 4. smt.
+have ->: W64x4.modulusR = W64x8.M ^ nlimbs. smt.
 rewrite W64x8.R.bn_mod. auto. 
 rewrite /bnk. 
 apply eq_big_seq. progress. rewrite H1. smt. auto.
 qed.
 
 
-
-lemma bn_expand_correct a  :
-  hoare[ M.bn_expand : arg = a  ==> W64x8.valR res = W64x4.valR a ].
-proc.
-sp. 
-seq 1 : (a = x /\ i = nlimbs /\ forall i, i < nlimbs => r.[i] = x.[i]%Array4).
-while (i <= nlimbs /\ forall j, 0 <= j < i => r.[j] = x.[j]%Array4). wp.  skip. progress.
-smt. smt. skip. progress.
-smt.  smt. smt. 
-seq 2 : (a = x /\  (forall j, 0 <= j < nlimbs => r.[j]%Array8 = x.[j]%Array4)
-     /\ (forall j, nlimbs <= j < 2*nlimbs => r.[j] = W64.zero)).     
-while (a = x /\ nlimbs <= i <= 2*nlimbs 
-     /\ (forall j, 0 <= j < nlimbs => r.[j]%Array8 = x.[j]%Array4)
-     /\ (forall j, nlimbs <= j < i => r.[j] = W64.zero) ). wp.  skip. progress.
-smt. smt.
-have z : i{hr} <> j. smt. 
-rewrite - H1. auto.  smt.
-case (j = i{hr}). smt.
-progress.
-have : j < i{hr}. timeout 10. smt.
-progress.
-rewrite - (H2 j).  smt.
-smt. wp. 
-skip.  progress.
-smt. smt. smt. 
-skip.  progress.
-have -> : valR r{hr} = (bn_seq ((to_list r{hr}))%Array8).
-apply W64x8.R.bn2seq. 
-rewrite /to_list.
-have -> : 8 = 4 + 4. smt().
-rewrite mkseq_add. auto. auto.
-have -> : mkseq (fun (i0 : int) => r{hr}.[i0]) nlimbs 
-  = mkseq (fun (i0 : int) => x{hr}.[i0]%Array4) nlimbs.
-apply eq_in_mkseq. progress. 
-simplify.
-have ->: mkseq (fun (i0 : int) => r{hr}.[nlimbs + i0]) nlimbs
-  = mkseq (fun (i0 : int) => W64.zero) nlimbs.
-apply eq_in_mkseq. progress. rewrite H0. smt. auto.
-rewrite mkseq_nseq. 
-rewrite /bn_seq.
-rewrite foldr_cat.
-have ->: (foldr (fun (w : W64.t) (r0 : int) => to_uint w + W64x8.M * r0) 0
-     (nseq nlimbs W64.zero)) = 0.  
-   have gen : forall n, 0 <= n => foldr (fun (w : W64.t) (r0 : int) => to_uint w + W64x8.M * r0) 0
-                 (nseq n  W64.zero) = 0.
-   apply intind. progress. rewrite nseq0. simplify. auto.
-   progress. rewrite nseqS. auto. search  foldr. simplify. rewrite H2. auto.
-   apply gen. auto.
-rewrite W64x4.R.bn2seq. rewrite /bn_seq. rewrite /to_list. 
-pose f := (fun (w : W64.t) (r0 : int) => to_uint w + W64x8.M * r0).
-simplify. auto.
-qed.
-
-lemma bn_expand_correct_ph a  :
-    phoare[ M.bn_expand : arg = a  ==> W64x8.valR res <> W64x4.valR a ] = 0%r.
-     hoare.
- conseq (bn_expand_correct a).
-qed.
-
-lemma bn_expand_correct_ph2 a  :
-    phoare[ M.bn_expand : arg = a  ==> W64x8.valR res =  W64x4.valR a ] = 1%r.
+lemma bn_expand_correct : forall a,
+      phoare[ M.bn_expand : arg = a  ==> W64x8.valR res =  W64x4.valR a ] = 1%r.
+ have  bn_expand_correct : forall a, 
+    hoare[ M.bn_expand : arg = a  ==> W64x8.valR res = W64x4.valR a ].
+   move => a.
+   proc.
+   sp. 
+    seq 1 : (a = x /\ i = nlimbs /\ forall i, i < nlimbs => r.[i] = x.[i]%Array4).
+    while (i <= nlimbs /\ forall j, 0 <= j < i => r.[j] = x.[j]%Array4). wp.  skip. progress.
+    smt. smt. skip. progress.
+    smt.  smt. smt. 
+    seq 2 : (a = x /\  (forall j, 0 <= j < nlimbs => r.[j]%Array8 = x.[j]%Array4)
+         /\ (forall j, nlimbs <= j < 2*nlimbs => r.[j] = W64.zero)).     
+    while (a = x /\ nlimbs <= i <= 2*nlimbs 
+         /\ (forall j, 0 <= j < nlimbs => r.[j]%Array8 = x.[j]%Array4)
+         /\ (forall j, nlimbs <= j < i => r.[j] = W64.zero) ). wp.  skip. progress.
+    smt. smt.
+    have z : i{hr} <> j. smt. 
+    rewrite - H1. auto.  smt.
+    case (j = i{hr}). smt.
+    progress.
+    have : j < i{hr}. timeout 10. smt.
+    progress.
+    rewrite - (H2 j).  smt.
+    smt. wp. 
+    skip.  progress.
+    smt. smt. smt. 
+    skip.  progress.
+    have -> : valR r{hr} = (bn_seq ((to_list r{hr}))%Array8).
+    apply W64x8.R.bn2seq. 
+    rewrite /to_list.
+    have -> : dnlimbs = nlimbs + nlimbs. smt().
+    rewrite mkseq_add. auto. auto.
+    have -> : mkseq (fun (i0 : int) => r{hr}.[i0]) nlimbs 
+      = mkseq (fun (i0 : int) => x{hr}.[i0]%Array4) nlimbs.
+    apply eq_in_mkseq. progress. 
+    simplify.
+    have ->: mkseq (fun (i0 : int) => r{hr}.[nlimbs + i0]) nlimbs
+      = mkseq (fun (i0 : int) => W64.zero) nlimbs.
+    apply eq_in_mkseq. progress. rewrite H0. smt. auto.
+    rewrite mkseq_nseq. 
+    rewrite /bn_seq.
+    rewrite foldr_cat.
+    have ->: (foldr (fun (w : W64.t) (r0 : int) => to_uint w + W64x8.M * r0) 0
+         (nseq nlimbs W64.zero)) = 0.  
+       have gen : forall n, 0 <= n => foldr (fun (w : W64.t) (r0 : int) => to_uint w + W64x8.M * r0) 0
+                     (nseq n  W64.zero) = 0.
+       apply intind. progress. rewrite nseq0. simplify. auto.
+       progress. rewrite nseqS. auto. search  foldr. simplify. rewrite H2. auto.
+       apply gen. auto.
+    rewrite W64x4.R.bn2seq. rewrite /bn_seq. rewrite /to_list. 
+    pose f := (fun (w : W64.t) (r0 : int) => to_uint w + W64x8.M * r0).
+    simplify. auto.    
+move => a.
 bypr. progress.
  have ->:  1%r = Pr[M.bn_expand(arg{m}) @ &m : true ] . 
 byphoare. proc.  while (true) (2*nlimbs -i). progress. wp. skip. smt().
@@ -341,59 +338,57 @@ wp.  skip. smt(). auto. auto.
   = Pr[M.bn_expand(arg{m}) @ &m : (W64x8.valR res =  W64x4.valR arg{m}) ]  + Pr[M.bn_expand(arg{m}) @ &m : (W64x8.valR res <>  W64x4.valR arg{m}) ].
 rewrite Pr[mu_split (W64x8.valR res =  W64x4.valR arg{m})]. simplify.   auto.
 have ->: Pr[M.bn_expand(arg{m}) @ &m : valR res <> valR arg{m}] = 0%r.
-byphoare (_: arg = arg{m} ==> _). conseq (bn_expand_correct_ph arg{m}). auto. auto. simplify. auto.
+byphoare (_: arg = arg{m} ==> _). 
+hoare. simplify. conseq (bn_expand_correct arg{m}). auto. auto. auto.
 qed.
 
 
 
-    
+
 equiv bnreduce_spec:
  M.bnreduce ~ CSpecFp.redm:
      W64x8.valR a{1} = a{2} 
  /\  W64x8.valR r{1} = r{2} 
  /\  W64x4.valR p{1} = P
- /\  k{2} = 256                 (* change that *)
+ /\  k{2} = 64 * nlimbs                 (* change that *)
    ==>  (W64x4.valR res{1}) = res{2}  %% W64x4.modulusR.
 proof. proc.
 sp.
 simplify.
-seq 0 0 : (valR a{1} = a{2} /\ valR r{1} = r{2} /\ ImplZZ p{1} P /\ k{2} = 256). skip. auto.
-seq 1 1 : (valR a{1} = a{2} /\ valR r{1} = r{2} /\ ImplZZ p{1} P /\ k{2} = 256
+seq 0 0 : (valR a{1} = a{2} /\ valR r{1} = r{2} /\ ImplZZ p{1} P /\ k{2} = 64 * nlimbs). skip. auto.
+seq 1 1 : (valR a{1} = a{2} /\ valR r{1} = r{2} /\ ImplZZ p{1} P /\ k{2} = 64 * nlimbs
     /\ W64x8.valR2 xr{1} = xr{2} (* /\ xr{2} = a{2} * r{2} *)).
 call dmuln_spec. skip. progress.
-seq 1 1 : (valR a{1} = a{2} /\ valR r{1} = r{2} /\ ImplZZ p{1} P /\ k{2} = 256
+seq 1 1 : (valR a{1} = a{2} /\ valR r{1} = r{2} /\ ImplZZ p{1} P /\ k{2} = 64 * nlimbs
     /\ W64x8.valR2 xr{1} = xr{2} /\ W64x8.valR xrf{1} = xrf{2} ).
-
-ecall {1} (bn_div2_correct xr{1}). inline*. wp.  skip.  progress.
-
-
-seq 1 1 : (valR a{1} = a{2} /\ valR r{1} = r{2} /\ ImplZZ p{1} P /\ k{2} = 256
+ecall {1} (bn_div2_correct xr{1}). inline*. wp.  skip.  progress. rewrite H0.
+  rewrite /W64x8.modulusR. clear H0 H. smt.
+seq 1 1 : (valR a{1} = a{2} /\ valR r{1} = r{2} /\ ImplZZ p{1} P /\ k{2} = 64 * nlimbs
     /\ W64x8.valR2 xr{1} = xr{2} /\  valR xrfd{1} =  xrf{2}   ).
 ecall {1} (bn_shrink_correct xrf{1}). wp. skip. progress. smt.
-
-seq 1 1 : (valR a{1} = a{2} /\ valR r{1} = r{2} /\ ImplZZ p{1} P /\ k{2} = 256
+seq 1 1 : (valR a{1} = a{2} /\ valR r{1} = r{2} /\ ImplZZ p{1} P /\ k{2} = 64 * nlimbs
     /\ W64x8.valR2 xr{1} = xr{2} /\ valR xrfd{1} = xrf{2} 
     /\  W64x8.valR xrfn{1} = xrfn{2}).
 call muln_spec. skip. progress.
-seq 1 1 : (valR a{1} = a{2} /\ valR r{1} = r{2} /\ ImplZZ p{1} P /\ k{2} = 256
+seq 1 1 : (valR a{1} = a{2} /\ valR r{1} = r{2} /\ ImplZZ p{1} P /\ k{2} = 64 * nlimbs
     /\ W64x8.valR2 xr{1} = xr{2} /\ W64x4.valR xrfd{1} = xrf{2} 
     /\ W64x8.valR xrfn{1} = xrfn{2}
     /\ W64x8.valR t{1} = t{2}).
 call dsubc_spec. skip. progress.
-seq 1 0 : (valR a{1} = a{2} /\ valR r{1} = r{2} /\ ImplZZ p{1} P /\ k{2} = 256
+seq 1 0 : (valR a{1} = a{2} /\ valR r{1} = r{2} /\ ImplZZ p{1} P /\ k{2} = 64 * nlimbs
     /\ W64x8.valR2 xr{1} = xr{2} /\ W64x4.valR xrfd{1} = xrf{2} 
     /\ W64x8.valR xrfn{1} = xrfn{2}
     /\ W64x8.valR t{1} = t{2}
     /\ W64x8.valR pp{1} = W64x4.valR p{1}).
-ecall {1} (bn_expand_correct_ph2 p{1} ). skip. progress.
-seq 1 1 : (valR a{1} = a{2} /\ valR r{1} = r{2} /\ ImplZZ p{1} P /\ k{2} = 256
+ecall {1} (bn_expand_correct p{1}). skip. progress.
+seq 1 1 : (valR a{1} = a{2} /\ valR r{1} = r{2} /\ ImplZZ p{1} P /\ k{2} = 64 * nlimbs
     /\ W64x8.valR2 xr{1} = xr{2} /\ W64x4.valR xrfd{1} = xrf{2} 
     /\ W64x8.valR xrfn{1} = xrfn{2}
     /\ W64x8.valR t{1} = t{2}
     /\ W64x8.valR pp{1} = W64x4.valR p{1}
     /\ W64x8.valR t{1} = t{2} ).
 call dcminusP_spec. skip. progress. smt().
-seq 1 0 : (valR a{1} = a{2} /\ valR r{1} = r{2} /\ ImplZZ p{1} P /\ k{2} = 256
+seq 1 0 : (valR a{1} = a{2} /\ valR r{1} = r{2} /\ ImplZZ p{1} P /\ k{2} = 64 * nlimbs
     /\ W64x8.valR2 xr{1} = xr{2} /\ W64x4.valR xrfd{1} = xrf{2} 
     /\ W64x8.valR xrfn{1} = xrfn{2}
     /\ W64x8.valR t{1} = t{2}
